theories/GeneralizeLtsOutputs.v
@@ -1,0 +1,338 @@
+(*
+   Copyright (c) 2024 Nomadic Labs
+   Copyright (c) 2024 Paul Laforgue <paul.laforgue@nomadic-labs.com>
+   Copyright (c) 2024 Léo Stefanesco <leo.stefanesco@mpi-sws.org>
+
+   Permission is hereby granted, free of charge, to any person obtaining a copy
+   of this software and associated documentation files (the "Software"), to deal
+   in the Software without restriction, including without limitation the rights
+   to use, copy, modify, merge, publish, distribute, sublicense, and/or sell
+   copies of the Software, and to permit persons to whom the Software is
+   furnished to do so, subject to the following conditions:
+
+   The above copyright notice and this permission notice shall be included in all
+   copies or substantial portions of the Software.
+
+   THE SOFTWARE IS PROVIDED "AS IS", WITHOUT WARRANTY OF ANY KIND, EXPRESS OR
+   IMPLIED, INCLUDING BUT NOT LIMITED TO THE WARRANTIES OF MERCHANTABILITY,
+   FITNESS FOR A PARTICULAR PURPOSE AND NONINFRINGEMENT. IN NO EVENT SHALL THE
+   AUTHORS OR COPYRIGHT HOLDERS BE LIABLE FOR ANY CLAIM, DAMAGES OR OTHER
+   LIABILITY, WHETHER IN AN ACTION OF CONTRACT, TORT OR OTHERWISE, ARISING FROM,
+   OUT OF OR IN CONNECTION WITH THE SOFTWARE OR THE USE OR OTHER DEALINGS IN THE
+   SOFTWARE.
+*)
+
+Require ssreflect.
+Require Import Coq.Unicode.Utf8.
+Require Import Coq.Lists.List.
+Import ListNotations.
+Require Import Coq.Program.Equality.
+Require Import Coq.Wellfounded.Inverse_Image.
+Require Import Coq.Logic.JMeq.
+Require Import Coq.Program.Wf Setoid.
+Require Import Coq.Program.Equality.
+From Coq.Logic Require Import ProofIrrelevance.
+
+From stdpp Require Import base countable list decidable finite gmap gmultiset.
+From Must Require Import TransitionSystems.
+
+(** Actions  *)
+
+Inductive ExtAct (A: Type) :=
+| ActIn (a : A)
+| ActOut (a : A)
+.
+Arguments ActIn {_} _.
+Arguments ActOut {_} _.
+
+Definition ext_act_match {A} (l1 l2: ExtAct A) :=
+  match l1, l2 with
+  | ActIn x, ActOut y => x = y
+  | ActOut x, ActIn y => x = y
+  | _, _ => False
+  end.
+
+Inductive Act (A: Type) :=
+| ActExt (μ: ExtAct A)
+| τ
+.
+Arguments ActExt {_} _.
+Arguments τ {_}.
+
+Definition co {A} (l: ExtAct A) :=
+  match l with
+  | ActIn x => ActOut x
+  | ActOut x => ActIn x
+  end.
+
+Lemma co_involution {A} (l: ExtAct A) : co (co l) = l.
+Proof. destruct l; eauto. Qed.
+
+Definition ext_match_commutative {A} (l1 l2: ExtAct A):
+  ext_act_match l1 l2 -> ext_act_match l2 l1.
+Proof. by destruct l1 as [?|?], l2 as [?|?]; eauto; intros ->. Qed.
+
+#[global] Instance actext_eqdec `{EqDecision L} : EqDecision (ExtAct L).
+Proof. solve_decision. Defined.
+#[global] Instance act_eqdec `{EqDecision L} : EqDecision (Act L).
+Proof. solve_decision. Defined.
+#[global] Instance ext_act_match_dec `{EqDecision L} : ∀ (ℓ1 ℓ2: ExtAct L), Decision (ext_act_match ℓ1 ℓ2).
+Proof.
+  intros [l1|l1] [l2|l2]; [by right; intros ? | | | by right; intros ?];
+    destruct (decide (l1 = l2)); eauto.
+Defined.
+
+Definition trace L := list (ExtAct L).
+
+Definition is_input {A} (μ : ExtAct A) := ∃ a, μ = ActIn a.
+
+Definition are_inputs {A} (s : trace A) := Forall is_input s.
+
+Definition is_output {A} (μ : ExtAct A) := ∃ a, μ = ActOut a.
+
+Definition are_outputs {A} (s : trace A) := Forall is_output s.
+
+
+Class Label (L: Type) :=
+  MkLabel {
+      label_eqdec: EqDecision L;
+      label_countable: Countable L;
+    }.
+#[global] Existing Instance label_eqdec.
+#[global] Existing Instance label_countable.
+
+Class Lts (A L : Type) `{Label L} :=
+  MkLts {
+      lts_step: A → Act L → A → Prop;
+      lts_state_eqdec: EqDecision A;
+
+      lts_step_decidable a α b : Decision (lts_step a α b);
+
+      lts_outputs : A -> gset L;
+      lts_outputs_spec1 p1 x p2 : lts_step p1 (ActExt (ActOut x)) p2 -> x ∈ lts_outputs p1;
+      lts_outputs_spec2 p1 x : x ∈ lts_outputs p1 -> {p2 | lts_step p1 (ActExt (ActOut x)) p2};
+
+      lts_stable: A → Act L → Prop;
+      lts_stable_decidable p α : Decision (lts_stable p α);
+      lts_stable_spec1 p α : ¬ lts_stable p α → { q | lts_step p α q };
+      lts_stable_spec2 p α : { q | lts_step p α q } → ¬ lts_stable p α;
+    }.
+#[global] Existing Instance lts_state_eqdec.
+#[global] Existing Instance lts_step_decidable.
+#[global] Existing Instance lts_stable_decidable.
+
+Notation "p ⟶ q"      := (lts_step p τ q) (at level 30, format "p  ⟶  q").
+Notation "p ⟶{ α } q" := (lts_step p α q) (at level 30, format "p  ⟶{ α }  q").
+Notation "p ⟶[ μ ] q" := (lts_step p (ActExt μ) q) (at level 30, format "p  ⟶[ μ ]  q").
+
+Notation "p ↛"      := (lts_stable p τ) (at level 30, format "p  ↛").
+Notation "p ↛{ α }" := (lts_stable p α) (at level 30, format "p  ↛{ α }").
+Notation "p ↛[ μ ]" := (lts_stable p (ActExt μ)) (at level 30, format "p  ↛[ μ ]").
+
+Class FiniteLts A L `{Lts A L} :=
+  MkFlts {
+      folts_states_countable: Countable A;
+      folts_next_states_finite p α : Finite (dsig (fun q => lts_step p α q));
+}.
+
+#[global] Existing Instance folts_states_countable.
+#[global] Existing Instance folts_next_states_finite.
+
+Class LtsEq (A L : Type) `{Lts A L} := {
+    (* todo: use Equivalence *)
+    eq_rel : A -> A -> Prop;
+    eq_rel_refl p : eq_rel p p;
+    eq_symm p q : eq_rel p q -> eq_rel q p;
+    eq_trans p q r : eq_rel p q -> eq_rel q r -> eq_rel p r;
+    (* reference: L 1.4.15 p.51 Sangiorgi pi-book *)
+    eq_spec p q (α : Act L) : (exists r, eq_rel p r /\ r ⟶{α} q) -> (exists r, p ⟶{α} r /\ eq_rel r q);
+  }.
+
+Add Parametric Relation `{Lts A L, ! LtsEq A L} : A eq_rel
+    reflexivity proved by (eq_rel_refl)
+    symmetry proved by (eq_symm)
+    transitivity proved by (eq_trans)
+    as sc_proc_rel.
+
+Infix "⋍" := eq_rel (at level 70).
+
+Definition lts_sc `{Lts A L, !LtsEq A L} p α q := exists r, p ⟶{α} r /\ r ⋍ q.
+
+Notation "p ⟶⋍ q" := (lts_sc p τ q) (at level 30, format "p  ⟶⋍  q").
+Notation "p ⟶⋍{ α } q" := (lts_sc p α q) (at level 30, format "p  ⟶⋍{ α }  q").
+Notation "p ⟶⋍[ μ ] q" := (lts_sc p (ActExt μ) q) (at level 30, format "p  ⟶⋍[ μ ]  q").
+
+Class LtsOba (A L : Type) `{Lts A L, !LtsEq A L} :=
+  MkOBA {
+      (* Multiset of outputs *)
+      lts_oba_mo p : gmultiset L;
+      lts_oba_mo_spec1 p a : a ∈ lts_oba_mo p <-> a ∈ lts_outputs p;
+      lts_oba_mo_spec2 p a : forall q, p ⟶[ActOut a] q -> lts_oba_mo p = {[+ a +]} ⊎ lts_oba_mo q;
+      (* Selinger axioms. *)
+      lts_oba_output_commutativity {p q r a α} :
+      p ⟶[ActOut a] q -> q ⟶{α} r -> (∃ t, p ⟶{α} t /\ t ⟶⋍[ActOut a] r) ;
+      lts_oba_output_confluence {p q1 q2 a μ} :
+      μ ≠ ActOut a -> p ⟶[ActOut a] q1 -> p ⟶[μ] q2 ->
+      ∃ r, q1 ⟶[μ] r /\ q2 ⟶⋍[ActOut a] r ;
+      lts_oba_output_tau {p q1 q2 a} :
+      p ⟶[ActOut a] q1 -> p ⟶ q2 -> (∃ t, q1 ⟶ t /\ q2 ⟶⋍[ActOut a] t) \/ q1 ⟶⋍[ActIn a] q2 ;
+      lts_oba_output_deter {p1 p2 p3 a} :
+      p1 ⟶[ActOut a] p2 -> p1 ⟶[ActOut a] p3 -> p2 ⋍ p3 ;
+      (* Extra axiom, it would be nice to remove it, not used that much. *)
+      lts_oba_output_deter_inv {p1 p2 q1 q2} a :
+      p1 ⟶[ActOut a] q1 -> p2 ⟶[ActOut a] q2 -> q1 ⋍ q2 -> p1 ⋍ p2
+    }.
+
+Class LtsObaFB (A L: Type) `{LtsOba A L} :=
+  MkLtsObaFB {
+      lts_oba_fb_feedback {p1 p2 p3 a} : p1 ⟶[ActOut a] p2 -> p2 ⟶[ActIn a] p3 -> p1 ⟶⋍ p3
+    }.
+
+Class LtsObaFW (A L : Type) `{LtsOba A L} :=
+  MkLtsObaFW {
+      lts_oba_fw_forward p1 a : ∃ p2, p1 ⟶[ActIn a] p2 /\ p2 ⟶[ActOut a] p1 ;
+      lts_oba_fw_feedback {p1 p2 p3 a} : p1 ⟶[ActOut a] p2 -> p2 ⟶[ActIn a] p3 -> p1 ⟶⋍ p3 \/ p1 ⋍ p3 ;
+    }.
+
+
+(* Genarilization via essential actions, non_blocking actions *)
+
+#[global] Instance ext_act_match_sym `{Label A} : Symmetric (@ext_act_match A).
+Proof. 
+  unfold ext_act_match.
+  intros μ1 μ2 Hyp.
+  destruct μ1; destruct μ2; eauto.
+Qed.
+
+Lemma simplify_match_output `{Label A} a μ : @ext_act_match A (ActOut a) μ <-> μ = ActIn a.
+Proof.
+  split.
+  + intros eq.
+    unfold ext_act_match in eq.
+    destruct μ; subst; eauto; try contradiction.
+  + intro. subst. simpl. eauto.
+Qed.
+
+Lemma simplify_match_input `{Label A} a μ : @ext_act_match A (ActIn a) μ <-> μ = ActOut a.
+Proof.
+  split.
+  + intros eq.
+    unfold ext_act_match in eq.
+    destruct μ; subst; eauto; try contradiction.
+  + intro. subst. simpl. eauto.
+Qed.
+
+#[global] Program Instance gLabel
+  `{Label A} : TransitionSystems.ExtAction (ExtAct A).
+Next Obligation.
+  intros. admit.
+Admitted.
+Next Obligation.
+  intros L H μ. exact (is_output μ).
+Defined.
+Next Obligation.
+ intros. destruct a.
+ + right. intro imp. destruct imp as (μ & eq). subst. inversion eq.
+ + left. exists a. eauto.
+Defined.
+Next Obligation.
+  intros A H μ1. exact (co μ1).
+Defined.
+Next Obligation.
+  intros. unfold relation. exact ext_act_match.
+Defined.
+Next Obligation.
+  intros. unfold sc. unfold gLabel_obligation_5.
+  destruct a; destruct b.
+  + right. intro cases. eauto. destruct cases as [case_1 | case_2].
+    ++ eapply simplify_match_input in case_1. inversion case_1.
+    ++ eapply simplify_match_input in case_2. inversion case_2.
+  + destruct (decide (a = a0)) as [eq1 | eq2].
+    ++ subst. left. left. simpl. eauto.
+    ++ subst. right. intro cases.
+       destruct cases as [case_1 | case_2].
+       +++ eapply simplify_match_input in case_1. inversion case_1. eauto.
+       +++ eapply simplify_match_output in case_2. inversion case_2. eauto.
+  + destruct (decide (a = a0)) as [eq1 | eq2].
+    ++ subst. left. left. simpl. eauto.
+    ++ subst. right. intro cases.
+       destruct cases as [case_1 | case_2].
+       +++ eapply simplify_match_output in case_1. inversion case_1. eauto.
+       +++ eapply simplify_match_input in case_2. inversion case_2. eauto.
+  + simpl in *. right. intro Hyp. destruct Hyp; eauto.
+Defined.
+Next Obligation.
+  intros. exists (co η). unfold sc. 
+  unfold gLabel_obligation_5. unfold ext_act_match.
+  destruct η; simpl in *; eauto. 
+Defined.
+Next Obligation. 
+  unfold sc. unfold gLabel_obligation_2.
+  unfold gLabel_obligation_5.
+  intros ? ? ? ? ? (a & eq) Hyp Hyp'. subst.
+  destruct Hyp as [case_1 | case_2]; destruct Hyp' as [case_1' | case_2']; exists a; eauto.
+  + eapply simplify_match_output in case_1. subst.
+    symmetry in case_1'. eapply simplify_match_input in case_1'. subst.
+    eauto.
+  + eapply simplify_match_output in case_1. subst.
+    eapply simplify_match_input. eauto.
+  + symmetry in case_2. eapply simplify_match_output in case_2. subst.
+    symmetry in case_1'. eapply simplify_match_input in case_1'. subst.
+    eauto.
+  + symmetry in case_2.
+    eapply simplify_match_output in case_2. subst.
+    eapply simplify_match_input in case_2'. subst.
+    eauto.
+Qed.
+Next Obligation.
+  unfold gLabel_obligation_2.
+  unfold gLabel_obligation_5.
+  intros A H η μ IsOut eq.
+  intro IsOut'. destruct IsOut' as (μ' & eq'); subst.
+  unfold sc in eq.
+  destruct eq as [eq_1 | eq_2].
+  + symmetry in eq_1.
+    eapply simplify_match_output in eq_1. subst.
+    destruct IsOut as ( a & impossible).
+    inversion impossible.
+  + eapply simplify_match_output in eq_2. subst.
+    destruct IsOut as ( a & impossible).
+    inversion impossible.
+Qed.
+Next Obligation.
+  unfold gLabel_obligation_2.
+  unfold gLabel_obligation_5.
+  unfold sc. unfold gLabel_obligation_4.
+  intros A H η μ IsOut eq.
+  destruct IsOut as (η' & eq'); subst.
+  destruct eq as [eq_1 | eq_2].
+  + eapply simplify_match_output in eq_1. subst. simpl. eauto.
+  + symmetry in eq_2.
+    eapply simplify_match_output in eq_2. subst. simpl. eauto.
+Qed.
+
+
+#[global] Program Instance gLts
+  `{LtsP: Lts P A} : TransitionSystems.Lts P A :=
+  {|
+    lts_step := lts_step;
+  |}.
+Next Obligation.
+Admitted.
+Next Obligation.
+Admitted.
+Next Obligation.
+Admitted.
+Next Obligation.
+Admitted.
+Next Obligation.
+Admitted.
+Next Obligation.
+Admitted.
+Next Obligation.
+Admitted.
+
+
+
+
+
