theories/Subset_Act.v
@@ -39,7 +39,7 @@ From Must Require Import TransitionSystems.
 Definition subset_of (A : Type) := A -> Prop.
 
 Definition lts_pre_acc_set_of `{Lts P A} (p : P) (μ : A) : Prop := 
-      ¬ lts_stable p (ActExt μ).
+      ¬ lts_refuses p (ActExt μ).
 
 Definition lts_acc_set_of `{Lts P A} (p : P) : subset_of A := lts_pre_acc_set_of p.
 
@@ -104,9 +104,9 @@ repeat split; try set_solver.
 #[global] Instance TopSet_of_Actions {A : Type} : TopSet A (@subset_of A).
 repeat split ; try set_solver. Defined.
 
-Lemma set_ind_L `{H : ExtAction A} (P : subset_of A) `{∀ x, Decision (P x)} : 
+(* Lemma set_ind_L `{H : ExtAction A} (P : subset_of A) `{∀ x, Decision (P x)} : 
   P ∅ → True. (∀ x X, x ∉ X → P X → P ({[ x ]} ∪ X)) → ∀ X, P X.
-Proof. apply set_ind. by intros ?? ->%leibniz_equiv_iff. Qed.
+Proof. apply set_ind. by intros ?? ->%leibniz_equiv_iff. Qed. *)
 
 (* Axiom Extensionality_Subset_of: 
   forall A : Type, forall S S': subset_of A, (S ⊆ S' /\ S' ⊆ S) -> S = S'.
